\documentclass[a4paper,12pt]{article}

\usepackage{array}
\usepackage{graphicx}
\usepackage{color}
\usepackage{colortbl}
\usepackage[export]{adjustbox}
\usepackage{multirow}
\usepackage{amssymb,amsmath}
% \usepackage[most]{tcolorbox}

\usepackage{tikz}
\usepackage{ctable}
\usetikzlibrary{shapes.misc,shadows}

\usepackage{geometry}
 \geometry{
 a4paper,
 total={210mm,297mm},
 left=20mm,
 right=20mm,
 top=16mm,
 bottom=15mm,
 }


\newcommand{\Conv}{%
  \mathop{\scalebox{1.5}{\raisebox{-0.2ex}{$\circledast$}}
  }
}

\newcommand{\Add}{%
  \mathop{\scalebox{1.5}{\raisebox{-0.2ex}{$\oplus$}}
  }
}

\begin{document}

\begin{equation*}
\begin{aligned}
& h^{sum}_{1} = x_1 * w_1 + x_2 * w_2 + b_1 \\
& h^{sum}_{2} = x_1 * w_3 + x_2 * w_4 + b_2
\end{aligned}
\end{equation*}
\\[1cm]
\begin{equation*}
\sigma(x) = \frac{1}{1 + e^{-x}}
\end{equation*}
\\[1cm]

\begin{equation*}
\begin{aligned}
& h_{1} = \sigma(h^{sum}_{1}) = \frac{1}{1 + e^{-h^{sum}_{1}}}\\[0.2cm]
& h_{2} = \sigma(h^{sum}_{2}) = \frac{1}{1 + e^{-h^{sum}_{2}}}
\end{aligned}
\end{equation*}
\\[1cm]

\begin{equation*}
\begin{aligned}
o^{sum}_{1} = h_{1} * w_5 + h_{2} * w_6 + b_3 \\
o_{1} = \sigma(o^{sum}_{1}) = \frac{1}{1 + e^{-o^{sum}_{1}}}
\end{aligned}
\end{equation*}
\\[1cm]

\begin{equation*}
\begin{aligned}
L &= \frac{1}{1}\sum_{i=1}^1{(y_i - \hat{y}_i)^2} \\
  &= (y_{true} - y_{pred})^2 \\
  &= (1 - 0.9824945598864127)^2 \\
  &= 0.0003064404335703929
\end{aligned}
\end{equation*}
\\[1cm]

\begin{equation*}
\begin{aligned}
L &= (y_{true} - y_{pred})^2
\end{aligned}
\end{equation*}
\\[1cm]

\begin{equation*}
\begin{aligned}
L &= L(y_{pred})
\end{aligned}
\end{equation*}

\begin{equation*}
\begin{aligned}
y_{pred} &= o_1 \\
         &= \sigma(o^{sum}_{1}) \\
         &= \frac{1}{1 + e^{-o^{sum}_{1}}} \\
         &= \frac{1}{1 + e^{-(h_{1} * w_5 + h_{2} * w_6 + b_3)}} \\
         &= \frac{1}{1 + e^{-\Big(\frac{1}{1 + e^{-h^{sum}_{1}}} * w_5 + \frac{1}{1 + e^{-h^{sum}_{2}}} * w_6 + b_3\Big)}} \\
         &= \frac{1}{1 + e^{-\Big(\frac{1}{1 + e^{-(x_1 * w_1 + x_2 * w_2 + b_1)}} * w_5 + \frac{1}{1 + e^{-(x_1 * w_3 + x_2 * w_4 + b_2)}} * w_6 + b_3\Big)}}
\end{aligned}
\end{equation*}

\begin{equation*}
\begin{aligned}
L &= L(y_{pred}) = L(w_1, w_2, w_3, w_4, w_5, w_6, b_1, b_2, b_3)
\end{aligned}
\end{equation*}
\\[1cm]

\begin{equation*}
\begin{aligned}
&\frac{\partial{L}}{\partial{w_i}}, \quad (i = 1, 2, 3, 4, 5, 6) \\
&\frac{\partial{L}}{\partial{b_j}}, \quad (j = 1, 2, 3)
\end{aligned}
\end{equation*}

\begin{equation*}
\begin{aligned}
&w_i = w_i - \eta * \frac{\partial{L}}{\partial{w_i}}, \quad (i = 1, 2, 3, 4, 5, 6) \\
&b_j = b_j - \eta * \frac{\partial{L}}{\partial{b_j}}, \quad (j = 1, 2, 3)
\end{aligned}
\end{equation*}
where, $\eta$ is a constant and it is called \textbf{learning rate}.

\begin{equation*}
\begin{aligned}
y_{pred} &= o_1 \\
         % &= \sigma(o^{sum}_{1}) \\
         % &= \frac{1}{1 + e^{-o^{sum}_{1}}} \\
y_{pred} &= \frac{1}{1 + e^{-(h_{1} * w_5 + h_{2} * w_6 + b_3)}}
         % &= \frac{1}{1 + e^{-\Big(\frac{1}{1 + e^{-h^{sum}_{1}}} * w_5 + \frac{1}{1 + e^{-h^{sum}_{2}}} * w_6 + b_3\Big)}} \\
         % &= \frac{1}{1 + e^{-\Big(\frac{1}{1 + e^{-(x_1 * w_1 + x_2 * w_2 + b_1)}} * w_5 + \frac{1}{1 + e^{-(x_1 * w_3 + x_2 * w_4 + b_2)}} * w_6 + b_3\Big)}}
\end{aligned}
\end{equation*}

\begin{equation*}
\begin{aligned}
\frac{\partial{L}}{\partial{w_1}} &= \frac{\partial{L}}{\partial{y_{pred}}}\frac{\partial{y_{pred}}}{\partial{w_1}} \\
                                  &= -2(y_{true} - y_{pred})\frac{\partial{y_{pred}}}{\partial{w_1}} \\[0.2cm]
\frac{\partial{y_{pred}}}{\partial{w_1}} &= \frac{\partial{y_{pred}}}{\partial{h_1}}\frac{\partial{h_1}}{\partial{w_1}} \\[0.2cm]
                                         &= \frac{\partial{\Big(\frac{1}{1 + e^{-(h_{1} * w_5 + h_{2} * w_6 + b_3)}}\Big)}}{\partial{h_1}}\frac{\partial{h_1}}{\partial{w_1}} \\[0.2cm]
                                         &= \frac{\partial{\Big(\frac{1}{1 + e^{-(h_{1} * w_5 + h_{2} * w_6 + b_3)}}\Big)}}{\partial{(h_{1} * w_5 + h_{2} * w_6 + b_3)}}\frac{\partial{(h_{1} * w_5 + h_{2} * w_6 + b_3)}}{\partial{h_1}}\frac{\partial{h_1}}{\partial{w_1}} \\[0.2cm]
                                         &= w_5\frac{\partial{\Big(\frac{1}{1 + e^{-(h_{1} * w_5 + h_{2} * w_6 + b_3)}}\Big)}}{\partial{(h_{1} * w_5 + h_{2} * w_6 + b_3)}}\frac{\partial{h_1}}{\partial{w_1}} \\[0.2cm]
                                         &= w_5\frac{\partial{\sigma(o^{sum}_{1})}}{\partial{o^{sum}_{1}}}\frac{\partial{h_1}}{\partial{w_1}} \\
\end{aligned}
\end{equation*}
\\[1cm]

\begin{equation*}
\begin{aligned}
\frac{\partial{\sigma(o^{sum}_{1})}}{\partial{o^{sum}_{1}}} &= \sigma'(o^{sum}_{1}) = \sigma(o^{sum}_{1})(1 - \sigma(o^{sum}_{1})) \\[0.3cm]
\frac{\partial{y_{pred}}}{\partial{w_1}} &= w_5\sigma'(o^{sum}_{1})\frac{\partial{h_1}}{\partial{w_1}} \\
                                         &= w_5\sigma'(o^{sum}_{1})\frac{\partial{h_1}}{\partial{h^{sum}_1}}\frac{\partial{h^{sum}_1}}{\partial{w_1}} \\
                                         &= w_5\sigma'(o^{sum}_{1})\frac{\partial{\sigma(h^{sum}_{1})}}{\partial{h^{sum}_1}}\frac{\partial{h^{sum}_1}}{\partial{w_1}} \\
                                         &= w_5\sigma'(o^{sum}_{1})\sigma'(h^{sum}_{1})\frac{\partial{h^{sum}_1}}{\partial{w_1}} \\
                                         &= w_5\sigma'(o^{sum}_{1})\sigma'(h^{sum}_{1})x_1 \\
\end{aligned}
\end{equation*}


\begin{equation*}
\begin{aligned}
\frac{\partial{L}}{\partial{w_1}} &= -2(y_{true} - y_{pred})w_5\sigma'(o^{sum}_{1})\sigma'(h^{sum}_{1})x_1
\end{aligned}
\end{equation*}


\begin{equation*}
\begin{aligned}
\frac{\partial{L}}{\partial{w_2}} &= -2(y_{true} - y_{pred})w_5\sigma'(o^{sum}_{1})\sigma'(h^{sum}_{1})x_2 \\
\frac{\partial{L}}{\partial{w_3}} &= -2(y_{true} - y_{pred})w_6\sigma'(o^{sum}_{1})\sigma'(h^{sum}_{2})x_1 \\
\frac{\partial{L}}{\partial{w_4}} &= -2(y_{true} - y_{pred})w_6\sigma'(o^{sum}_{1})\sigma'(h^{sum}_{2})x_2 \\[0.3cm]
\frac{\partial{L}}{\partial{w_5}} &= -2(y_{true} - y_{pred})\sigma'(o^{sum}_{1})h_1 \\
\frac{\partial{L}}{\partial{w_6}} &= -2(y_{true} - y_{pred})\sigma'(o^{sum}_{1})h_2 \\[0.3cm]
\frac{\partial{L}}{\partial{b_1}} &= -2(y_{true} - y_{pred})w_5\sigma'(o^{sum}_{1})\sigma'(h^{sum}_{1}) \\
\frac{\partial{L}}{\partial{b_2}} &= -2(y_{true} - y_{pred})w_6\sigma'(o^{sum}_{1})\sigma'(h^{sum}_{2}) \\
\frac{\partial{L}}{\partial{b_3}} &= -2(y_{true} - y_{pred})\sigma'(o^{sum}_{1}) \\
\end{aligned}
\end{equation*}

\[
g_1 \circledast g_2 \circledast \cdots \circledast g_n=\Conv_{i=1}^{n} g_i
\]

\[
\underbrace{g \circledast g \circledast \cdots \circledast g}_{m}=g^{\circledast m}
\]

$\Conv$

$\Add$\\[0.2cm]

$\sigma$\\[0.3cm]

$\boldsymbol{b}^1$\\[0.2cm]
$\boldsymbol{b}^2$\\[0.2cm]
$\boldsymbol{k}^1$\\[0.2cm]
$\boldsymbol{k}^2$\\[0.2cm]
$\boldsymbol{w}$\\[0.2cm]
$\boldsymbol{b}$\\[0.2cm]
$\odot$\\[0.2cm]

% \tcbox[enhanced,colback=white]{\Large ReLU}

$\boldsymbol{o}$\\[0.2cm]

\begin{equation*}
\begin{bmatrix}
o_{0}\\
o_{1}\\
o_{2}\\
o_{3}\\
o_{4}\\
o_{5}\\
o_{6}\\
o_{7}\\
o_{8}\\
o_{9}\\
\end{bmatrix}
\end{equation*}
\\[0.2cm]
$\boldsymbol{C}^1$\\[0.2cm]
$\boldsymbol{C}^2$\\[0.2cm]
$\boldsymbol{P}^1$\\[0.2cm]
$\boldsymbol{P}^2$\\[0.2cm]
$k^1_{m,n,1}$\\[0.2cm]
$k^1_{m,n,2}$\\[0.2cm]
$k^1_{m,n,6}$\\[0.2cm]
$k^2_{m,n,1}$\\[0.2cm]
$k^2_{m,n,2}$\\[0.2cm]
$k^2_{m,n,3}$\\[0.2cm]
$b^1_1$\\[0.2cm]
$b^1_2$\\[0.2cm]
$b^1_6$\\[0.2cm]
$b^2_1$\\[0.2cm]
$b^2_2$\\[0.2cm]
$C^1_{g,h,1}$\\[0.2cm]
$C^1_{g,h,2}$\\[0.2cm]
$C^1_6$\\[0.2cm]
$C^2_{p,q,1}$\\[0.2cm]
$P^1_{r,s,1}$\\[0.2cm]
$P^1_{r,s,2}$\\[0.2cm]
$P^2_{u,v,1}$\\[0.2cm]

\begin{tikzpicture}[baseline=(char.base)]
\node(char)[draw,fill=white,
  shape=circle,
  minimum width=0cm]
  {$\boldsymbol{V}$};
\end{tikzpicture}

\end{document}